progress

BlockCacheSystem/BlockCacheSystem_Refines_TSJBlockInterface.i.dfy
@@ -25,7 +25,7 @@ module BlockCacheSystem_Refines_TSJBlockInterface {
   // that BetreeBlockCacheSystem refines TSJPivotBetree.
 
   import opened G = PivotBetreeGraph
-  import BCS = BetreeGraphBlockCacheSystem
+  import BCS = BlockCacheSystem
   import opened AsyncSectorDiskModelTypes
 
   import opened Maps
@@ -33,7 +33,7 @@ module BlockCacheSystem_Refines_TSJBlockInterface {
   import opened Options
   import opened NativeTypes
 
-  import BC = BetreeGraphBlockCache
+  import BC = BlockCache
   import BI = PivotBetreeBlockInterface
   import D = AsyncSectorDisk
   import ThreeState = ThreeStateTypes
@@ -53,13 +53,13 @@ module BlockCacheSystem_Refines_TSJBlockInterface {
   function EphemeralGraph(k: BCS.Constants, s: BCS.Variables) : imap<Reference, Node>
   requires BCS.Inv(k, s)
   {
-    MapToImap(EphemeralGraph(k, s))
+    MapToImap(BCS.EphemeralGraph(k, s))
   }
 
   function FrozenGraph(k: BCS.Constants, s: BCS.Variables) : imap<Reference, Node>
   requires BCS.Inv(k, s)
   {
-    MapToImap(EphemeralGraph(k, s))
+    MapToImap(BCS.FrozenGraph(k, s))
   }
 
   predicate CommitOccurredNotAcked(s: BCS.Variables)
@@ -90,6 +90,44 @@ module BlockCacheSystem_Refines_TSJBlockInterface {
     map id | 0 <= id < 0x1_0000_0000_0000_0000 && id as uint64 in s.machine.syncReqs :: SyncReqState(k, s, s.machine.syncReqs[id as uint64])
   }
 
+  predicate IsFreezeStep(k: BCS.Constants, s: BCS.Variables, step: BCS.Step)
+  {
+    && step.MachineStep?
+    && (
+      || step.machineStep.FreezeStep?
+      || (
+        && step.machineStep.WriteBackJournalReqStep?
+        && s.machine.Ready?
+        && s.machine.inMemoryJournalFrozen == []
+      )
+      || (
+        && step.machineStep.WriteBackJournalReqWraparoundStep?
+        && s.machine.Ready?
+        && s.machine.inMemoryJournalFrozen == []
+      )
+    )
+  }
+
+  predicate IsCrashStep(k: BCS.Constants, s: BCS.Variables, step: BCS.Step)
+  {
+    && step.CrashStep?
+  }
+
+  predicate IsPersistStep(k: BCS.Constants, s: BCS.Variables, step: BCS.Step)
+  {
+    && step.DiskInternalStep?
+    && step.step.ProcessWriteStep?
+    && BCS.ProcessWriteIsGraphUpdate(k, s, step.step.id)
+  }
+
+  predicate IsAdvanceLogStep(k: BCS.Constants, s: BCS.Variables, step: BCS.Step)
+  {
+    && step.DiskInternalStep?
+    && step.step.ProcessWriteStep?
+    && BCS.ProcessWriteIsSuperblockUpdate(k, s, step.step.id)
+    && !BCS.ProcessWriteIsGraphUpdate(k, s, step.step.id)
+  }
+
   predicate IsTransactionStep(step: BCS.Step)
   {
     && step.MachineStep?
@@ -101,6 +139,8 @@ module BlockCacheSystem_Refines_TSJBlockInterface {
     s: BCS.Variables,
     s': BCS.Variables)
   {
+    && BCS.Inv(k, s)
+    && BCS.Inv(k, s')
     && PersistentGraph(k, s') == PersistentGraph(k, s)
     && FrozenGraph(k, s') == FrozenGraph(k, s)
     && EphemeralGraph(k, s') == EphemeralGraph(k, s)
@@ -111,11 +151,30 @@ module BlockCacheSystem_Refines_TSJBlockInterface {
     && BCS.DeltaJournal(s') == BCS.DeltaJournal(s)
   }
 
+  predicate UpdateCrash(
+    k: BCS.Constants,
+    s: BCS.Variables,
+    s': BCS.Variables)
+  {
+    && BCS.Inv(k, s)
+    && BCS.Inv(k, s')
+    && PersistentGraph(k, s') == PersistentGraph(k, s)
+    && FrozenGraph(k, s') == PersistentGraph(k, s)
+    && EphemeralGraph(k, s') == PersistentGraph(k, s)
+    && BCS.PersistentJournal(s') == BCS.PersistentJournal(s)
+    && BCS.FrozenJournal(s') == BCS.PersistentJournal(s)
+    && BCS.EphemeralJournal(s') == BCS.PersistentJournal(s)
+    && BCS.GammaJournal(s') == BCS.PersistentJournal(s)
+    && BCS.DeltaJournal(s') == []
+  }
+
   predicate UpdateMove1to2(
     k: BCS.Constants,
     s: BCS.Variables,
     s': BCS.Variables)
   {
+    && BCS.Inv(k, s)
+    && BCS.Inv(k, s')
     && PersistentGraph(k, s') == FrozenGraph(k, s)
     && FrozenGraph(k, s') == FrozenGraph(k, s)
     && EphemeralGraph(k, s') == EphemeralGraph(k, s)
@@ -131,11 +190,13 @@ module BlockCacheSystem_Refines_TSJBlockInterface {
     s: BCS.Variables,
     s': BCS.Variables)
   {
-    && PersistentGraph(k, s') == FrozenGraph(k, s)
+    && BCS.Inv(k, s)
+    && BCS.Inv(k, s')
+    && PersistentGraph(k, s') == PersistentGraph(k, s)
     && FrozenGraph(k, s') == EphemeralGraph(k, s)
     && EphemeralGraph(k, s') == EphemeralGraph(k, s)
-    && BCS.PersistentJournal(s') == BCS.FrozenJournal(s)
-    && BCS.FrozenJournal(s') == BCS.EphemeralJournal(s)
+    && BCS.PersistentJournal(s') == BCS.PersistentJournal(s)
+    && BCS.FrozenJournal(s') == []
     && BCS.EphemeralJournal(s') == BCS.EphemeralJournal(s)
     && BCS.GammaJournal(s') == BCS.GammaJournal(s) + BCS.DeltaJournal(s)
     && BCS.DeltaJournal(s') == []
@@ -146,6 +207,8 @@ module BlockCacheSystem_Refines_TSJBlockInterface {
     s: BCS.Variables,
     s': BCS.Variables)
   {
+    && BCS.Inv(k, s)
+    && BCS.Inv(k, s')
     && PersistentGraph(k, s') == PersistentGraph(k, s)
     && FrozenGraph(k, s') == FrozenGraph(k, s)
     && EphemeralGraph(k, s') == EphemeralGraph(k, s)
@@ -159,8 +222,15 @@ module BlockCacheSystem_Refines_TSJBlockInterface {
   predicate UpdateUnalloc(
     k: BCS.Constants,
     s: BCS.Variables,
-    s': BCS.Variables)
+    s': BCS.Variables,
+    step: BCS.Step)
   {
+    && BCS.Inv(k, s)
+    && BCS.Inv(k, s')
+
+    && step.MachineStep?
+    && step.machineStep.UnallocStep?
+
     && PersistentGraph(k, s') == PersistentGraph(k, s)
     && FrozenGraph(k, s') == FrozenGraph(k, s)
     && EphemeralGraph(k, s') == IMapRemove1(EphemeralGraph(k, s), step.machineStep.ref)
@@ -178,34 +248,60 @@ module BlockCacheSystem_Refines_TSJBlockInterface {
     step: BCS.Step)
   requires IsTransactionStep(step)
   {
+    && BCS.Inv(k, s)
+    && BCS.Inv(k, s')
+
+    && step.MachineStep?
+    && step.machineStep.TransactionStep?
+    && step.machineStep.journalStep.JSNew?
+
     && PersistentGraph(k, s') == PersistentGraph(k, s)
     && FrozenGraph(k, s') == FrozenGraph(k, s)
     && BI.OpTransaction(BI.Constants(),
             BI.Variables(EphemeralGraph(k, s)),
             BI.Variables(EphemeralGraph(k, s')),
             step.machineStep.ops)
-    && BCS.PersistentJournal(s') == BCS.GammaJournal(s)
+    && BCS.PersistentJournal(s') == BCS.PersistentJournal(s)
     && BCS.FrozenJournal(s') == BCS.FrozenJournal(s)
     && BCS.EphemeralJournal(s) == []
     && BCS.EphemeralJournal(s') == []
     && BCS.GammaJournal(s') == BCS.GammaJournal(s)
-    && BCS.DeltaJournal(s') == step.machineStep.newJournal
+    && BCS.DeltaJournal(s') == BCS.DeltaJournal(s) + step.machineStep.journalStep.entries
   }
 
-  lemma InitImpliesGraphsEq(k: BCS.Constants, s: BCS.Variables)
-  requires BCS.Init(k, s)
-  ensures PersistentGraph(k, s) == FrozenGraph(k, s)
-  ensures PersistentGraph(k, s) == EphemeralGraph(k, s)
+  predicate ReplayTransaction(
+    k: BCS.Constants,
+    s: BCS.Variables,
+    s': BCS.Variables,
+    step: BCS.Step)
+  requires IsTransactionStep(step)
   {
-    reveal_PersistentGraph();
-    reveal_FrozenGraph();
-    reveal_EphemeralGraph();
+    && BCS.Inv(k, s)
+    && BCS.Inv(k, s')
+
+    && step.MachineStep?
+    && step.machineStep.TransactionStep?
+    && step.machineStep.journalStep.JSReplay?
+
+    && PersistentGraph(k, s') == PersistentGraph(k, s)
+    && FrozenGraph(k, s') == FrozenGraph(k, s)
+    && BI.OpTransaction(BI.Constants(),
+            BI.Variables(EphemeralGraph(k, s)),
+            BI.Variables(EphemeralGraph(k, s')),
+            step.machineStep.ops)
+    && BCS.PersistentJournal(s') == BCS.PersistentJournal(s)
+    && BCS.FrozenJournal(s') == BCS.FrozenJournal(s)
+    && BCS.GammaJournal(s') == BCS.GammaJournal(s)
+    && BCS.DeltaJournal(s') == BCS.DeltaJournal(s)
+    && step.machineStep.journalStep.entries + BCS.EphemeralJournal(s')
+        == BCS.EphemeralJournal(s)
   }
 
-  lemma TransactionUpdate(k: BCS.Constants, s: BCS.Variables, s': BCS.Variables, ops: seq<Op>)
+
+  lemma OpTransactionUpdate(k: BCS.Constants, s: BCS.Variables, s': BCS.Variables, ops: seq<Op>)
   requires BCS.Inv(k, s)
   requires s.disk == s'.disk
-  requires BC.Transaction(k.machine, s.machine, s'.machine, D.NoDiskOp, ops)
+  requires BC.OpTransaction(k.machine, s.machine, s'.machine, ops)
   ensures BCS.Inv(k, s')
   ensures PersistentGraph(k, s') == PersistentGraph(k, s)
   ensures FrozenGraph(k, s') == FrozenGraph(k, s)
@@ -213,30 +309,51 @@ module BlockCacheSystem_Refines_TSJBlockInterface {
             BI.Variables(EphemeralGraph(k, s)),
             BI.Variables(EphemeralGraph(k, s')),
             ops)
+  ensures BCS.PersistentJournal(s') == BCS.PersistentJournal(s)
+  ensures BCS.FrozenJournal(s') == BCS.FrozenJournal(s)
+  ensures BCS.EphemeralJournal(s') == BCS.EphemeralJournal(s)
+  ensures BCS.GammaJournal(s') == BCS.GammaJournal(s)
+  ensures BCS.DeltaJournal(s') == BCS.DeltaJournal(s)
+
   ensures SyncReqs(k, s) == SyncReqs(k, s');
   decreases |ops|
   {
-    reveal_PersistentGraph();
-    reveal_FrozenGraph();
-    reveal_EphemeralGraph();
+    //reveal_PersistentGraph();
+    //reveal_FrozenGraph();
+    //reveal_EphemeralGraph();
     if |ops| == 0 {
     } else if |ops| == 1 {
+      BCS.OpPreservesInv(k, s, s', ops[0]);
       reveal_SyncReqs();
       match ops[0] {
         case WriteOp(ref, block) => {
           BCS.DirtyStepUpdatesGraph(k, s, s', ref, block);
+          BCS.DirtyStepPreservesJournals(k, s, s', ref, block);
           assert s.machine.syncReqs == s'.machine.syncReqs;
+          assert BI.Write(BI.Constants(),
+              BI.Variables(EphemeralGraph(k, s)),
+              BI.Variables(EphemeralGraph(k, s')),
+              ref, block);
+          assert BI.OpStep(BI.Constants(),
+              BI.Variables(EphemeralGraph(k, s)),
+              BI.Variables(EphemeralGraph(k, s')),
+              ops[0]);
         }
         case AllocOp(ref, block) => {
           BCS.AllocStepUpdatesGraph(k, s, s', ref, block);
+          BCS.AllocStepPreservesJournals(k, s, s', ref, block);
           assert s.machine.syncReqs == s'.machine.syncReqs;
+          assert BI.OpStep(BI.Constants(),
+              BI.Variables(EphemeralGraph(k, s)),
+              BI.Variables(EphemeralGraph(k, s')),
+              ops[0]);
         }
       }
     } else {
       var ops1, mid, ops2 := BC.SplitTransaction(k.machine, s.machine, s'.machine, ops);
       var smid := AsyncSectorDiskModelVariables(mid, s.disk);
-      TransactionUpdate(k, s, smid, ops1);
-      TransactionUpdate(k, smid, s', ops2);
+      OpTransactionUpdate(k, s, smid, ops1);
+      OpTransactionUpdate(k, smid, s', ops2);
       BI.JoinTransactions(BI.Constants(),
         BI.Variables(EphemeralGraph(k, s)),
         BI.Variables(EphemeralGraph(k, smid)),
@@ -245,19 +362,43 @@ module BlockCacheSystem_Refines_TSJBlockInterface {
     }
   }
 
+  lemma TransactionUpdate(k: BCS.Constants, s: BCS.Variables, s': BCS.Variables, step: BCS.Step)
+  requires BCS.Inv(k, s)
+  requires s.disk == s'.disk
+  requires step.MachineStep?
+  requires step.machineStep.TransactionStep?
+  requires BC.Transaction(k.machine, s.machine, s'.machine, D.NoDiskOp, step.machineStep.ops, step.machineStep.journalStep)
+
+  ensures BCS.Inv(k, s')
+  ensures step.machineStep.journalStep.JSNew? ==>
+      UpdateTransaction(k, s, s', step)
+  ensures step.machineStep.journalStep.JSReplay? ==>
+      ReplayTransaction(k, s, s', step)
+
+  ensures SyncReqs(k, s) == SyncReqs(k, s');
+  {
+    var s1 := s.(machine := BC.DoJournalStep(s.machine, step.machineStep.journalStep));
+    BCS.JournalStepPreservesGraphs(k, s, s1, step.machineStep.journalStep);
+    BCS.JournalStepPreservesJournals(k, s, s1, step.machineStep.journalStep);
+    OpTransactionUpdate(k, s1, s', step.machineStep.ops);
+
+    assert SyncReqs(k, s) == SyncReqs(k, s1) by { reveal_SyncReqs(); }
+  }
+
   lemma RefinesReads(k: BCS.Constants, s: BCS.Variables, ops: seq<ReadOp>)
   requires BCS.Inv(k, s)
   requires BC.Reads(k.machine, s.machine, ops)
   ensures BI.Reads(BI.Constants(), BI.Variables(EphemeralGraph(k, s)), ops)
   {
-    reveal_EphemeralGraph();
-    /*forall op | op in ops
+    //reveal_EphemeralGraph();
+    forall op | op in ops
     ensures BI.ReadStep(BI.Constants, BI.Variables(EphemeralGraph(k, s)), op)
     {
-      assert s.machine.cache[op.ref] == op.node;
-      assert op.ref in EphemeralGraph(k, s);
-      assert EphemeralGraph(k, s)[op.ref] == op.node;
-    }*/
+      BCS.EphemeralGraphRead(k, s, op);
+      //assert s.machine.cache[op.ref] == op.node;
+      //assert op.ref in EphemeralGraph(k, s);
+      //assert EphemeralGraph(k, s)[op.ref] == op.node;
+    }
   }
 
   lemma UnallocStepMeetsGCConditions(k: BCS.Constants, s: BCS.Variables, s': BCS.Variables,
@@ -267,7 +408,8 @@ module BlockCacheSystem_Refines_TSJBlockInterface {
   requires BC.Unalloc(k.machine, s.machine, s'.machine, dop, ref)
   ensures BI.CanGCRefs(BI.Constants(), BI.Variables(EphemeralGraph(k, s)), iset{ref})
   {
-    reveal_EphemeralGraph();
+    BCS.UnallocStepUpdatesGraph(k, s, s', dop, ref);
+    //reveal_EphemeralGraph();
     if (ref in BI.LiveReferences(BI.Constants(), BI.Variables(EphemeralGraph(k, s)))) {
       assert BI.ReachableReference(BI.Constants(), BI.Variables(EphemeralGraph(k, s)), ref);
       var lookup :| BI.LookupIsValid(BI.Constants(), BI.Variables(EphemeralGraph(k, s)), lookup) && Last(lookup) == ref;
@@ -286,63 +428,180 @@ module BlockCacheSystem_Refines_TSJBlockInterface {
   requires BCS.NextStep(k, s, s', step)
   ensures BCS.Inv(k, s')
 
-  ensures !IsTransactionStep(step) ==> (
-      || UpdateAllEq(k, s, s')
-      || UpdateMove1to2(k, s, s')
+  ensures IsFreezeStep(k, s, step) ==>
       || UpdateMove2to3(k, s, s')
       || UpdateExtendLog(k, s, s')
-      || UpdateUnalloc(k, s, s')
-    )
 
-  ensures (step.MachineStep? && step.machineStep.TransactionStep? ==>
-      && PersistentGraph(k, s') == PersistentGraph(k, s)
-      && FrozenGraph(k, s') == FrozenGraph(k, s)
-      && BI.OpTransaction(BI.Constants(),
-            BI.Variables(EphemeralGraph(k, s)),
-            BI.Variables(EphemeralGraph(k, s')),
-            step.machineStep.ops)
-    )
+  ensures IsCrashStep(k, s, step) ==>
+      UpdateCrash(k, s, s')
 
-  ensures (step.MachineStep? && step.machineStep.UnallocStep? ==>
-      && PersistentGraph(k, s') == PersistentGraph(k, s)
-      && FrozenGraph(k, s') == FrozenGraph(k, s)
-      && EphemeralGraph(k, s') == IMapRemove1(EphemeralGraph(k, s), step.machineStep.ref)
+  ensures IsPersistStep(k, s, step) ==>
+      UpdateMove1to2(k, s, s')
+
+  ensures IsAdvanceLogStep(k, s, step) ==>
+      UpdateExtendLog(k, s, s')
+
+  ensures IsTransactionStep(step) ==> (
+    && (step.machineStep.journalStep.JSNew? ==>
+        UpdateTransaction(k, s, s', step))
+    && (step.machineStep.journalStep.JSReplay? ==>
+        ReplayTransaction(k, s, s', step))
+  )
+
+  ensures (
+      && !IsTransactionStep(step)
+      && !IsFreezeStep(k, s, step)
+      && !IsPersistStep(k, s, step)
+      && !IsAdvanceLogStep(k, s, step)
+      && !IsCrashStep(k, s, step)
+    ) ==> (
+      || UpdateAllEq(k, s, s')
+      || UpdateUnalloc(k, s, s', step)
     )
   {
     BCS.NextStepPreservesInv(k, s, s', step);
 
-    reveal_PersistentGraph();
-    reveal_FrozenGraph();
-    reveal_EphemeralGraph();
+    //reveal_PersistentGraph();
+    //reveal_FrozenGraph();
+    //reveal_EphemeralGraph();
 
     match step {
       case MachineStep(dop, machineStep) => {
         match machineStep {
-          case WriteBackReqStep(ref) => BCS.WriteBackReqStepPreservesGraphs(k, s, s', dop, ref);
-          case WriteBackRespStep => BCS.WriteBackRespStepPreservesGraphs(k, s, s', dop);
-          case WriteBackIndirectionTableReqStep => BCS.WriteBackIndirectionTableReqStepPreservesGraphs(k, s, s', dop);
-          case WriteBackIndirectionTableRespStep => BCS.WriteBackIndirectionTableRespStepPreservesGraphs(k, s, s', dop);
-          case UnallocStep(ref: Reference) => BCS.UnallocStepUpdatesGraph(k, s, s', dop, ref);
-          case PageInReqStep(ref: Reference) => BCS.PageInReqStepPreservesGraphs(k, s, s', dop, ref);
-          case PageInRespStep => BCS.PageInRespStepPreservesGraphs(k, s, s', dop);
-          case PageInIndirectionTableReqStep => BCS.PageInIndirectionTableReqStepPreservesGraphs(k, s, s', dop);
-          case PageInIndirectionTableRespStep => BCS.PageInIndirectionTableRespStepPreservesGraphs(k, s, s', dop);
-          case EvictStep(ref: Reference) => BCS.EvictStepPreservesGraphs(k, s, s', dop, ref);
-          case FreezeStep => BCS.FreezeStepPreservesGraphs(k, s, s', dop);
-          case PushSyncReqStep(id) => BCS.PushSyncReqStepPreservesGraphs(k, s, s', dop, id);
-          case PopSyncReqStep(id) => BCS.PopSyncReqStepPreservesGraphs(k, s, s', dop, id);
-          case NoOpStep => { }
-          case TransactionStep(ops) => TransactionUpdate(k, s, s', ops);
+          case WriteBackReqStep(ref) => {
+            BCS.WriteBackReqStepPreservesGraphs(k, s, s', dop, ref);
+            BCS.WriteBackReqStepPreservesJournals(k, s, s', dop, ref);
+          }
+          case WriteBackRespStep => {
+            BCS.WriteBackRespStepPreservesGraphs(k, s, s', dop);
+            BCS.WriteBackRespStepPreservesJournals(k, s, s', dop);
+          }
+          case WriteBackIndirectionTableReqStep => {
+            BCS.WriteBackIndirectionTableReqStepPreservesGraphs(k, s, s', dop);
+            BCS.WriteBackIndirectionTableReqStepPreservesJournals(k, s, s', dop);
+          }
+          case WriteBackIndirectionTableRespStep => {
+            BCS.WriteBackIndirectionTableRespStepPreservesGraphs(k, s, s', dop);
+            BCS.WriteBackIndirectionTableRespStepPreservesJournals(k, s, s', dop);
+          }
+          case WriteBackJournalReqStep(jr) => {
+            BCS.WriteBackJournalReqStepPreservesGraphs(k, s, s', dop, jr);
+            BCS.WriteBackJournalReqStepPreservesJournals(k, s, s', dop, jr);
+            if IsFreezeStep(k, s, step) {
+              assert UpdateExtendLog(k, s, s');
+            } else {
+              assert UpdateAllEq(k, s, s');
+            }
+          }
+          case WriteBackJournalReqWraparoundStep(jr) => {
+            BCS.WriteBackJournalReqWraparoundStepPreservesGraphs(k, s, s', dop, jr);
+            BCS.WriteBackJournalReqWraparoundStepPreservesJournals(k, s, s', dop, jr);
+          }
+          case WriteBackJournalRespStep => {
+            BCS.WriteBackJournalRespStepPreservesGraphs(k, s, s', dop);
+            BCS.WriteBackJournalRespStepPreservesJournals(k, s, s', dop);
+          }
+          case WriteBackSuperblockReq_Basic_Step => {
+            BCS.WriteBackSuperblockReq_Basic_StepPreservesGraphs(k, s, s', dop);
+            BCS.WriteBackSuperblockReq_Basic_StepPreservesJournals(k, s, s', dop);
+          }
+          case WriteBackSuperblockReq_UpdateIndirectionTable_Step => {
+            BCS.WriteBackSuperblockReq_UpdateIndirectionTable_StepPreservesGraphs(k, s, s', dop);
+            BCS.WriteBackSuperblockReq_UpdateIndirectionTable_StepPreservesJournals(k, s, s', dop);
+          }
+          case WriteBackSuperblockRespStep => {
+            BCS.WriteBackSuperblockRespStepPreservesGraphs(k, s, s', dop);
+            BCS.WriteBackSuperblockRespStepPreservesJournals(k, s, s', dop);
+          }
+          case UnallocStep(ref: Reference) => {
+            BCS.UnallocStepUpdatesGraph(k, s, s', dop, ref);
+            BCS.UnallocStepPreservesJournals(k, s, s', dop, ref);
+          }
+          case PageInReqStep(ref: Reference) => {
+            BCS.PageInReqStepPreservesGraphs(k, s, s', dop, ref);
+            BCS.PageInReqStepPreservesJournals(k, s, s', dop, ref);
+          }
+          case PageInRespStep => {
+            BCS.PageInRespStepPreservesGraphs(k, s, s', dop);
+            BCS.PageInRespStepPreservesJournals(k, s, s', dop);
+          }
+          case PageInIndirectionTableReqStep => {
+            BCS.PageInIndirectionTableReqStepPreservesGraphs(k, s, s', dop);
+            BCS.PageInIndirectionTableReqStepPreservesJournals(k, s, s', dop);
+          }
+          case PageInIndirectionTableRespStep => {
+            BCS.PageInIndirectionTableRespStepPreservesGraphs(k, s, s', dop);
+            BCS.PageInIndirectionTableRespStepPreservesJournals(k, s, s', dop);
+          }
+          case PageInJournalReqStep(which) => {
+            BCS.PageInJournalReqStepPreservesGraphs(k, s, s', dop, which);
+            BCS.PageInJournalReqStepPreservesJournals(k, s, s', dop, which);
+          }
+          case PageInJournalRespStep(which) => {
+            BCS.PageInJournalRespStepPreservesGraphs(k, s, s', dop, which);
+            BCS.PageInJournalRespStepPreservesJournals(k, s, s', dop, which);
+          }
+          case PageInSuperblockReqStep(which) => {
+            BCS.PageInSuperblockReqStepPreservesGraphs(k, s, s', dop, which);
+            BCS.PageInSuperblockReqStepPreservesJournals(k, s, s', dop, which);
+          }
+          case PageInSuperblockRespStep(which) => {
+            BCS.PageInSuperblockRespStepPreservesGraphs(k, s, s', dop, which);
+            BCS.PageInSuperblockRespStepPreservesJournals(k, s, s', dop, which);
+          }
+          case FinishLoadingSuperblockPhaseStep => {
+            BCS.FinishLoadingSuperblockPhaseStepPreservesGraphs(k, s, s', dop);
+            BCS.FinishLoadingSuperblockPhaseStepPreservesJournals(k, s, s', dop);
+          }
+          case FinishLoadingOtherPhaseStep => {
+            BCS.FinishLoadingOtherPhaseStepPreservesGraphs(k, s, s', dop);
+            BCS.FinishLoadingOtherPhaseStepPreservesJournals(k, s, s', dop);
+          }
+          case EvictStep(ref: Reference) => {
+            BCS.EvictStepPreservesGraphs(k, s, s', dop, ref);
+            BCS.EvictStepPreservesJournals(k, s, s', dop, ref);
+          }
+          case FreezeStep => {
+            BCS.FreezeStepPreservesGraphs(k, s, s', dop);
+            BCS.FreezeStepPreservesJournals(k, s, s', dop);
+            assert UpdateMove2to3(k, s, s');
+          }
+          case PushSyncReqStep(id) => {
+            BCS.PushSyncReqStepPreservesGraphs(k, s, s', dop, id);
+            BCS.PushSyncReqStepPreservesJournals(k, s, s', dop, id);
+          }
+          case PopSyncReqStep(id) => {
+            BCS.PopSyncReqStepPreservesGraphs(k, s, s', dop, id);
+            BCS.PopSyncReqStepPreservesJournals(k, s, s', dop, id);
+          }
+          case NoOpStep => {
+            BCS.NoOpStepPreservesGraphs(k, s, s', dop);
+            BCS.NoOpStepPreservesJournals(k, s, s', dop);
+          }
+          case TransactionStep(ops, js) => TransactionUpdate(k, s, s', step);
         }
       }
-      case DiskInternalStep(step) => {
-        match step {
-          case ProcessReadStep(id) => BCS.ProcessReadPreservesGraphs(k, s, s', id);
-          case ProcessReadFailureStep(id) => BCS.ProcessReadFailurePreservesGraphs(k, s, s', id);
-          case ProcessWriteStep(id) => BCS.ProcessWritePreservesGraphs(k, s, s', id);
+      case DiskInternalStep(disk_step) => {
+        match disk_step {
+          case ProcessReadStep(id) => {
+            BCS.ProcessReadPreservesGraphs(k, s, s', id);
+            BCS.ProcessReadPreservesJournals(k, s, s', id);
+          }
+          case ProcessReadFailureStep(id) => {
+            BCS.ProcessReadFailurePreservesGraphs(k, s, s', id);
+            BCS.ProcessReadFailurePreservesJournals(k, s, s', id);
+          }
+          case ProcessWriteStep(id) => {
+            BCS.ProcessWritePreservesGraphs(k, s, s', id);
+            BCS.ProcessWritePreservesJournals(k, s, s', id);
+          }
         }
       }
-      case CrashStep => { }
+      case CrashStep => {
+        BCS.CrashPreservesGraphs(k, s, s');
+        BCS.CrashPreservesJournals(k, s, s');
+        assert UpdateCrash(k, s, s');
+      }
     }
   }
 
@@ -352,7 +611,7 @@ module BlockCacheSystem_Refines_TSJBlockInterface {
   ensures BCS.Inv(k, s')
 
   ensures IsPersistStep(k, s, step) ==> SyncReqs(k, s') == ThreeState.SyncReqs2to1(SyncReqs(k, s))
-  ensures IsFreezeStep(step) ==> SyncReqs(k, s') == ThreeState.SyncReqs3to2(SyncReqs(k, s))
+  ensures IsFreezeStep(k, s, step) ==> SyncReqs(k, s') == ThreeState.SyncReqs3to2(SyncReqs(k, s))
   ensures step.MachineStep? && step.machineStep.PushSyncReqStep? ==>
       && step.machineStep.id as int !in SyncReqs(k, s)
       && SyncReqs(k, s') == SyncReqs(k, s)[step.machineStep.id as int := ThreeState.State3]
@@ -363,7 +622,7 @@ module BlockCacheSystem_Refines_TSJBlockInterface {
   ensures step.CrashStep? ==> SyncReqs(k, s') == map[]
   ensures
     && !IsPersistStep(k, s, step)
-    && !IsFreezeStep(step)
+    && !IsFreezeStep(k, s, step)
     && !step.CrashStep?
     && !(step.MachineStep? && step.machineStep.PushSyncReqStep?)
     && !(step.MachineStep? && step.machineStep.PopSyncReqStep?)
@@ -374,7 +633,7 @@ module BlockCacheSystem_Refines_TSJBlockInterface {
 
     if (
       && !IsPersistStep(k, s, step)
-      && !IsFreezeStep(step)
+      && !IsFreezeStep(k, s, step)
       && !step.CrashStep?
       && !(step.MachineStep? && step.machineStep.PushSyncReqStep?)
       && !(step.MachineStep? && step.machineStep.PopSyncReqStep?)
@@ -410,8 +669,8 @@ module BlockCacheSystem_Refines_TSJBlockInterface {
             case PushSyncReqStep(id) => assert SyncReqs(k,s) == SyncReqs(k,s');
             case PopSyncReqStep(id) => assert SyncReqs(k,s) == SyncReqs(k,s');
             case NoOpStep => assert SyncReqs(k,s) == SyncReqs(k,s');
-            case TransactionStep(ops) => {
-              TransactionUpdate(k, s, s', ops);
+            case TransactionStep(ops, js) => {
+              TransactionUpdate(k, s, s', step);
               assert SyncReqs(k,s) == SyncReqs(k,s');
             }
           }
